theory/x64Assembler.thy
@@ -23,7 +23,7 @@ fun x64_assemble_one_instruction :: "instruction \<Rightarrow> x64_bin option" w
     let (op:: u8) = 0x89 in
     let (rop::u8) = construct_modsib_to_u8 0b11 (u8_of_ireg r1) (u8_of_ireg rd) in
       Some [ rex, op, rop] |
-  \<comment> \<open> P2882 `MOV register1 to register2` -> `0100 1R0B : 1000 1001 : 11 reg1 reg2` \<close>
+  \<comment> \<open> P2882 `MOV qwordregister1 to qwordregister2` -> `0100 1R0B : 1000 1001 : 11 reg1 reg2` \<close>
   Pmovq_rr rd r1 \<Rightarrow>
     let (rex:: u8) = or 0x40 (construct_rex_to_u8  \<comment> \<open> `1R0B` \<close>
       True \<comment> \<open> W \<close>
