theory/x64ConsistencyProof1.thy
@@ -2,84 +2,138 @@ theory x64ConsistencyProof1
 imports
   Main
   rBPFCommType rBPFSyntax
-  x64Assembler x64Disassembler
+  x64Assembler x64Disassembler x64ConsistencyProof1Ins
 begin
-(*
-declare if_split_asm [split] *)
-
-(*
-lemma list_eq_rewrite: "x#y = l \<Longrightarrow> f l = f (x#y)" by auto *)
 
 
-value "x64_assemble [Pmov_rr ireg.R8 ireg.RAX]"
-(**r Some [102, 65, 137, 192] *)
-value "x64_disassemble [102, 65, 137, 192]"
+lemma x64assemble_disassemble_consistency:
+  "x64_assemble l_asm = Some l_bin \<Longrightarrow> x64_disassemble l_bin = Some l_asm"
+  apply (induction l_asm arbitrary: l_bin)
+   apply simp
 
-value "or (or 192 (u8_of_ireg ireg.RAX << 3)) x86CommType.RBX"
-(** 195 *)
-value "ireg_of_u8
-     (or (and x86CommType.RDI (and x86CommType.RCX (0 >> 2)))
-       (and (and x86CommType.RDI (195 >> 3)) (- x86CommType.R8)))"
-(**r Some ireg.RAX *)
+  subgoal for a l_asm l_bin
+    apply simp
+    apply (cases a, auto)
 
-value "and x86CommType.RBX (195 >> 6) = x86CommType.RBX"
+      \<comment> \<open> Pmovq_rr \<close>
+    subgoal for rd r1 using x64assemble_disassemble_consistency_pmovq_rr
+      by blast
+      \<comment> \<open> Pmovl_rr \<close>
+    subgoal for rd r1 using x64assemble_disassemble_consistency_pmovl_rr
+      by blast
+      \<comment> \<open> Pnegl \<close>
+    subgoal for rd using x64assemble_disassemble_consistency_pnegl
+      by blast
+      \<comment> \<open> Pnegq \<close>
+    subgoal for rd using x64assemble_disassemble_consistency_pnegq
+      by blast
+      \<comment> \<open> Paddq_rr \<close>
+    subgoal for rd r1 using x64assemble_disassemble_consistency_paddq_rr
+      by blast
+      \<comment> \<open> Paddl_rr \<close>
+    subgoal for rd r1 using x64assemble_disassemble_consistency_paddl_rr
+      by blast
+      \<comment> \<open> Psubl_rr \<close>
+    subgoal for rd r1 using x64assemble_disassemble_consistency_psubl_rr
+      by blast
+      \<comment> \<open> Psubq_rr \<close>
+    subgoal for rd r1 using x64assemble_disassemble_consistency_psubq_rr
+      by blast 
 
-(*
-lemma rbx_simp [simp]: "or (or 192 (and 56 (u8_of_ireg r1 << 3))) (and x86CommType.RDI (u8_of_ireg rd)) = rop
-  \<Longrightarrow> and x86CommType.RBX (rop >> 6) = x86CommType.RBX"
-  apply (cases r1; cases rd, auto)
-  done
+      \<comment> \<open> Pmull_r \<close>
+    subgoal for r1 using x64assemble_disassemble_consistency_pmull_r
+      by blast
+      \<comment> \<open> Pmulq_r \<close>
+    subgoal for r1 using x64assemble_disassemble_consistency_pmulq_r
+      by blast
+      \<comment> \<open> Pimull_r \<close>
+    subgoal for r1 using x64assemble_disassemble_consistency_pimull_r
+      by blast
+      \<comment> \<open> Pimulq_r \<close>
+    subgoal for r1 using x64assemble_disassemble_consistency_pimulq_r
+      by blast
+      \<comment> \<open> Pdivl_r \<close>
+    subgoal for r1 using x64assemble_disassemble_consistency_pdivl_r
+      by blast
+      \<comment> \<open> Pdivq_r \<close>
+    subgoal for r1 using x64assemble_disassemble_consistency_pdivq_r
+      by blast
+      \<comment> \<open> Pidivl_r \<close>
+    subgoal for r1 using x64assemble_disassemble_consistency_pidivl_r
+      by blast
+      \<comment> \<open> Pidivq_r \<close>
+    subgoal for r1 using x64assemble_disassemble_consistency_pidivq_r
+      by blast
 
-lemma pmov_src [simp]: "
-     prefix = 102 \<and>
-     or 64
-     (or (u8_of_bool (and (u8_of_ireg r1) x86CommType.R8 \<noteq> x86CommType.RAX) << 2)
-       (u8_of_bool (and (u8_of_ireg rd) x86CommType.R8 \<noteq> x86CommType.RAX))) =
-    rex \<and>
-    op = 137 \<and>
-    or (or 192 (and 56 (u8_of_ireg r1 << 3))) (and x86CommType.RDI (u8_of_ireg rd)) = rop \<and>
-    l2 = l1 \<Longrightarrow>
-    ireg_of_u8
-            (bitfield_insert_u8 3 (Suc 0) (and x86CommType.RDI (rop >> 3)) (and x86CommType.RCX (rex >> 2)))
-       = Some r1"
-  apply (unfold u8_of_bool_def bitfield_insert_u8_def Let_def)
-  apply (cases r1; cases rd, auto simp add: ireg_of_u8_def)
-  done *)
-
-lemma x64assemble_disassemble_consistency_pmovq_rr: "\<And>x11 x12.
-       (\<And>l_bin. x64_assemble l_asm = Some l_bin \<Longrightarrow> x64_disassemble l_bin = Some l_asm) \<Longrightarrow>
-       (case x64_assemble l_asm of None \<Rightarrow> None
-        | Some l \<Rightarrow>
-            Some
-             ([or 64 (construct_rex_to_u8 True (and (u8_of_ireg x12) 8 \<noteq> 0) False (and (u8_of_ireg x11) 8 \<noteq> 0)),
-               137, construct_modsib_to_u8 3 (u8_of_ireg x12) (u8_of_ireg x11)] @
-              l)) =
-       Some l_bin \<Longrightarrow>
-       a = Pmovq_rr x11 x12 \<Longrightarrow> x64_disassemble l_bin = Some (Pmovq_rr x11 x12 # l_asm)"
-  subgoal for rd r1
-    apply (cases "x64_assemble l_asm", simp_all)
-    subgoal for l1
-      apply (unfold construct_rex_to_u8_def construct_modsib_to_u8_def)
-      apply simp
-      apply (cases l_bin)
-      subgoal by fastforce
-      subgoal for rex l1
+      \<comment> \<open> Pandl_rr \<close>
+    subgoal for rd r1 using x64assemble_disassemble_consistency_pandl_rr
+      by blast
+      \<comment> \<open> Pandq_rr \<close>
+    subgoal for rd r1 using x64assemble_disassemble_consistency_pandq_rr
+      by blast
+      \<comment> \<open> Porl_rr \<close>
+    subgoal for rd r1 using x64assemble_disassemble_consistency_porl_rr
+      by blast
+      \<comment> \<open> Porq_rr \<close>
+    subgoal for rd r1 using x64assemble_disassemble_consistency_porq_rr
+      by blast
+      \<comment> \<open> Pxorl_rr \<close>
+    subgoal for rd r1 using x64assemble_disassemble_consistency_pxorl_rr
+      by blast
+      \<comment> \<open> Pxorq_rr \<close>
+    subgoal for rd r1 using x64assemble_disassemble_consistency_pxorq_rr
+      by blast
+      \<comment> \<open> Pshll_ri \<close>
+    subgoal for rd n using x64assemble_disassemble_consistency_pshll_ri
+      by blast
+      \<comment> \<open> Pshlq_ri \<close>
+    subgoal for rd n using x64assemble_disassemble_consistency_pshlq_ri
+      by blast
+      \<comment> \<open> Pshll_r \<close>
+    subgoal for rd using x64assemble_disassemble_consistency_pshll_r
+      by blast
+      \<comment> \<open> Pshlq_r \<close>
+    subgoal for rd  using x64assemble_disassemble_consistency_pshlq_r
+      by blast
+      \<comment> \<open> Pshrl_ri \<close>
+    subgoal for rd n using x64assemble_disassemble_consistency_pshrl_ri
+      by blast
+      \<comment> \<open> Pshrq_ri \<close>
+    subgoal for rd n using x64assemble_disassemble_consistency_pshrq_ri
+      by blast
+      \<comment> \<open> Pshrl_r \<close>
+    subgoal for rd using x64assemble_disassemble_consistency_pshrl_r
+      by blast
+      \<comment> \<open> Pshrq_r \<close>
+    subgoal for rd  using x64assemble_disassemble_consistency_pshrq_r
+      by blast
+      \<comment> \<open> Psarl_ri \<close>
+    subgoal for rd n using x64assemble_disassemble_consistency_psarl_ri
+      by blast
+      \<comment> \<open> Psarq_ri \<close>
+    subgoal for rd n using x64assemble_disassemble_consistency_psarq_ri
+      by blast
+      \<comment> \<open> Psarl_r \<close>
+    subgoal for rd  using x64assemble_disassemble_consistency_psarl_r
+      by blast
+      \<comment> \<open> Psarq_r \<close>
+    subgoal for rd  using x64assemble_disassemble_consistency_psarq_r
+      by blast
+      \<comment> \<open> pnop \<close>
+      apply (cases "x64_assemble l_asm")
+      subgoal by simp
+      subgoal for l1
         apply simp
-        apply (cases l1)
+        apply (cases l_bin)
         subgoal by fastforce
-        subgoal for op l1
+        subgoal for prefix l1
           apply simp
-          apply (cases l1)
-          subgoal by fastforce
-          subgoal for reg l1
-            apply simp
-            apply (cases r1; cases rd,auto simp add: bitfield_insert_u8_def Let_def ireg_of_u8_def)
-            done
           done
         done
       done
     done
-  done
+
+end
 
 \<comment> \<open> 
                 apply (frule conjunct2)
@@ -104,185 +158,45 @@ lemma x64assemble_disassemble_consistency_pmovq_rr: "\<And>x11 x12.
                 apply (auto simp add: bitfield_insert_u8_def Let_def ireg_of_u8_def split: ireg.split)\<close>
 
 
-lemma x64assemble_disassemble_consistency_pneg: "\<And>x21a.
-       (\<And>l_bin. x64_assemble l_asm = Some l_bin \<Longrightarrow> x64_disassemble l_bin = Some l_asm) \<Longrightarrow>
-       (case x64_assemble l_asm of None \<Rightarrow> None
-        | Some l \<Rightarrow>
-            Some
-             ([or 64 (construct_rex_to_u8 True False False (and (u8_of_ireg x21a) 8 \<noteq> 0)), 247,
-               construct_modsib_to_u8 3 3 (u8_of_ireg x21a)] @
-              l)) =
-       Some l_bin \<Longrightarrow>
-       a = Pnegq x21a \<Longrightarrow> x64_disassemble l_bin = Some (Pnegq x21a # l_asm)"
-  subgoal for rd
-    apply (cases "x64_assemble l_asm")
-    subgoal by simp
-    subgoal for l1
-      apply simp
-      apply (unfold construct_rex_to_u8_def construct_modsib_to_u8_def)
-      apply simp
-      apply (cases l_bin)
-      subgoal by fastforce
-      subgoal for rex l1
-        apply (cases l1)
-        subgoal by fastforce
-        subgoal for op l1
-          apply simp
-          apply (cases l1)
-          subgoal by fastforce
-          subgoal for reg l1
-            apply simp
-            apply (cases rd, auto simp add: bitfield_insert_u8_def Let_def ireg_of_u8_def)
-            done
-          done
-        done
-      done
-    done
+(*
+lemma rbx_simp [simp]: "or (or 192 (and 56 (u8_of_ireg r1 << 3))) (and x86CommType.RDI (u8_of_ireg rd)) = rop
+  \<Longrightarrow> and x86CommType.RBX (rop >> 6) = x86CommType.RBX"
+  apply (cases r1; cases rd, auto)
   done
 
-lemma x64assemble_disassemble_consistency_paddq_rr :"\<And>x221 x222.
-       (\<And>l_bin. x64_assemble l_asm = Some l_bin \<Longrightarrow> x64_disassemble l_bin = Some l_asm) \<Longrightarrow>
-       (case x64_assemble l_asm of None \<Rightarrow> None
-        | Some l \<Rightarrow>
-            Some
-             ([or 64 (construct_rex_to_u8 True (and (u8_of_ireg x222) 8 \<noteq> 0) False (and (u8_of_ireg x221) 8 \<noteq> 0)),
-               1, construct_modsib_to_u8 3 (u8_of_ireg x222) (u8_of_ireg x221)] @
-              l)) =
-       Some l_bin \<Longrightarrow>
-       a = Paddq_rr x221 x222 \<Longrightarrow> x64_disassemble l_bin = Some (Paddq_rr x221 x222 # l_asm)"
-  subgoal for rd r1
-    apply (cases "x64_assemble l_asm")
-    subgoal by simp
-    subgoal for l1
-      apply simp
-      apply (unfold construct_rex_to_u8_def construct_modsib_to_u8_def)
-      apply simp
-      apply (cases l_bin)
-      subgoal by fastforce
-      subgoal for rex l1
-        apply (cases l1)
-        subgoal by fastforce
-        subgoal for op l1
-          apply simp
-          apply (cases l1)
-          subgoal by fastforce
-          subgoal for reg l1
-            apply simp
-            apply (cases r1; cases rd, auto simp add: bitfield_insert_u8_def Let_def ireg_of_u8_def)
-            done
-          done
-        done
-      done
-    done
-  done
+lemma pmov_src [simp]: "
+     prefix = 102 \<and>
+     or 64
+     (or (u8_of_bool (and (u8_of_ireg r1) x86CommType.R8 \<noteq> x86CommType.RAX) << 2)
+       (u8_of_bool (and (u8_of_ireg rd) x86CommType.R8 \<noteq> x86CommType.RAX))) =
+    rex \<and>
+    op = 137 \<and>
+    or (or 192 (and 56 (u8_of_ireg r1 << 3))) (and x86CommType.RDI (u8_of_ireg rd)) = rop \<and>
+    l2 = l1 \<Longrightarrow>
+    ireg_of_u8
+            (bitfield_insert_u8 3 (Suc 0) (and x86CommType.RDI (rop >> 3)) (and x86CommType.RCX (rex >> 2)))
+       = Some r1"
+  apply (unfold u8_of_bool_def bitfield_insert_u8_def Let_def)
+  apply (cases r1; cases rd, auto simp add: ireg_of_u8_def)
+  done *)
 
-lemma x64assemble_disassemble_consistency_psubq_rr: "\<And>x251 x252.
-       (\<And>l_bin. x64_assemble l_asm = Some l_bin \<Longrightarrow> x64_disassemble l_bin = Some l_asm) \<Longrightarrow>
-       (case x64_assemble l_asm of None \<Rightarrow> None
-        | Some l \<Rightarrow>
-            Some
-             ([or 64 (construct_rex_to_u8 True (and (u8_of_ireg x252) 8 \<noteq> 0) False (and (u8_of_ireg x251) 8 \<noteq> 0)),
-               41, construct_modsib_to_u8 3 (u8_of_ireg x252) (u8_of_ireg x251)] @
-              l)) =
-       Some l_bin \<Longrightarrow>
-       a = Psubq_rr x251 x252 \<Longrightarrow> x64_disassemble l_bin = Some (Psubq_rr x251 x252 # l_asm)"
-  subgoal for rd r1
-    apply (cases "x64_assemble l_asm")
-    subgoal by simp
-    subgoal for l1
-      apply simp
-      apply (unfold construct_rex_to_u8_def construct_modsib_to_u8_def)
-      apply simp
-      apply (cases l_bin)
-      subgoal by fastforce
-      subgoal for rex l1
-        apply (cases l1)
-        subgoal by fastforce
-        subgoal for op l1
-          apply simp
-          apply (cases l1)
-          subgoal by fastforce
-          subgoal for reg l1
-            apply simp
-            apply (cases r1; cases rd, auto simp add: bitfield_insert_u8_def Let_def ireg_of_u8_def)
-            done
-          done
-        done
-      done
-    done
-  done
+(*(*
+declare if_split_asm [split] *)
 
-lemma x64assemble_disassemble_consistency:
-  "x64_assemble l_asm = Some l_bin \<Longrightarrow> x64_disassemble l_bin = Some l_asm"
-  apply (induction l_asm arbitrary: l_bin)
-   apply simp
+(*
+lemma list_eq_rewrite: "x#y = l \<Longrightarrow> f l = f (x#y)" by auto *)
 
-  subgoal for a l_asm l_bin
-    apply simp
-    apply (cases a, auto)
 
-      \<comment> \<open> Pmovq_rr \<close>
-    subgoal for rd r1 using x64assemble_disassemble_consistency_pmovq_rr
-      by blast
+value "x64_assemble [Pmov_rr ireg.R8 ireg.RAX]"
+(**r Some [102, 65, 137, 192] *)
+value "x64_disassemble [102, 65, 137, 192]"
 
-      \<comment> \<open> Pnegq \<close>
-    subgoal for rd using x64assemble_disassemble_consistency_pneg
-      by blast
+value "or (or 192 (u8_of_ireg ireg.RAX << 3)) x86CommType.RBX"
+(** 195 *)
+value "ireg_of_u8
+     (or (and x86CommType.RDI (and x86CommType.RCX (0 >> 2)))
+       (and (and x86CommType.RDI (195 >> 3)) (- x86CommType.R8)))"
+(**r Some ireg.RAX *)
 
-      \<comment> \<open> Paddq_rr \<close>
-    subgoal for rd using x64assemble_disassemble_consistency_paddq_rr
-      by blast
-      \<comment> \<open> Psubq_rr \<close>
-    subgoal for rd using x64assemble_disassemble_consistency_psubq_rr
-      by blast
-      \<comment> \<open> Pmull_r \<close>
-    subgoal  sorry
-      \<comment> \<open> Pmulq_r \<close>
-    subgoal  sorry
-      \<comment> \<open> Pimull_r \<close>
-    subgoal  sorry
-      \<comment> \<open> Pmulq_r \<close>
-    subgoal  sorry
-      \<comment> \<open> Pmulq_r \<close>
-    subgoal  sorry
-    subgoal  sorry
-      \<comment> \<open> Pmulq_r \<close>
-    subgoal  sorry
-      \<comment> \<open> Pmulq_r \<close>
-    subgoal  sorry
-    subgoal  sorry
-      \<comment> \<open> Pmulq_r \<close>
-    subgoal  sorry
-      \<comment> \<open> Pmulq_r \<close>
-    subgoal  sorry
-    subgoal  sorry
-      \<comment> \<open> Pmulq_r \<close>
-    subgoal  sorry
-      \<comment> \<open> Pmulq_r \<close>
-    subgoal  sorry
-    subgoal  sorry
-      \<comment> \<open> Pmulq_r \<close>
-    subgoal  sorry
-      \<comment> \<open> Pmulq_r \<close>
-    subgoal  sorry
-    subgoal  sorry
-      \<comment> \<open> Pmulq_r \<close>
-    subgoal  sorry
-      \<comment> \<open> Pmulq_r \<close>
-    subgoal  sorry
-
-      \<comment> \<open> pnop \<close>
-      apply (cases "x64_assemble l_asm")
-      subgoal by simp
-      subgoal for l1
-        apply simp
-        apply (cases l_bin)
-        subgoal by fastforce
-        subgoal for prefix l1
-          apply simp
-          done
-        done
-      done
-    done
-
-end
+value "and x86CommType.RBX (195 >> 6) = x86CommType.RBX"
+*)
