theory/x64ConsistencyProof1Ins.thy
@@ -1,0 +1,1256 @@
+theory x64ConsistencyProof1Ins
+imports
+  Main
+  rBPFCommType rBPFSyntax
+  x64Assembler x64Disassembler
+begin
+
+
+lemma x64assemble_disassemble_consistency_pmovq_rr: "\<And>x11 x12.
+       (\<And>l_bin. x64_assemble l_asm = Some l_bin \<Longrightarrow> x64_disassemble l_bin = Some l_asm) \<Longrightarrow>
+       (case x64_assemble l_asm of None \<Rightarrow> None
+        | Some l \<Rightarrow>
+            Some
+             ([or 64 (construct_rex_to_u8 True (and (u8_of_ireg x12) 8 \<noteq> 0) False (and (u8_of_ireg x11) 8 \<noteq> 0)),
+               137, construct_modsib_to_u8 3 (u8_of_ireg x12) (u8_of_ireg x11)] @
+              l)) =
+       Some l_bin \<Longrightarrow>
+       a = Pmovq_rr x11 x12 \<Longrightarrow> x64_disassemble l_bin = Some (Pmovq_rr x11 x12 # l_asm)"
+  subgoal for rd r1
+    apply (cases "x64_assemble l_asm", simp_all)
+    subgoal for l1
+      apply (unfold construct_rex_to_u8_def construct_modsib_to_u8_def)
+      apply simp
+      apply (cases l_bin)
+      subgoal by fastforce
+      subgoal for rex l1
+        apply simp
+        apply (cases l1)
+        subgoal by fastforce
+        subgoal for op l1
+          apply simp
+          apply (cases l1)
+          subgoal by fastforce
+          subgoal for reg l1
+            apply simp
+            apply (cases r1; cases rd,auto simp add: bitfield_insert_u8_def Let_def ireg_of_u8_def)
+            done
+          done
+        done
+      done
+    done
+  done
+
+
+
+lemma x64assemble_disassemble_consistency_pmovl_rr: "\<And>x21 x22.
+       (\<And>l_bin.
+           x64_assemble l_asm = Some l_bin \<Longrightarrow> x64_disassemble l_bin = Some l_asm) \<Longrightarrow>
+       (case x64_assemble l_asm of None \<Rightarrow> None
+        | Some l \<Rightarrow>
+            Some
+             ([or 64
+                (construct_rex_to_u8 False (and (u8_of_ireg x22) 8 \<noteq> 0) False
+                  (and (u8_of_ireg x21) 8 \<noteq> 0)),
+               137, construct_modsib_to_u8 3 (u8_of_ireg x22) (u8_of_ireg x21)] @
+              l)) =
+       Some l_bin \<Longrightarrow>
+       a = Pmovl_rr x21 x22 \<Longrightarrow> x64_disassemble l_bin = Some (Pmovl_rr x21 x22 # l_asm)"
+  subgoal for rd r1
+    apply (cases "x64_assemble l_asm", simp_all)
+    subgoal for l1
+      apply (unfold construct_rex_to_u8_def construct_modsib_to_u8_def)
+      apply simp
+      apply (cases l_bin)
+      subgoal by fastforce
+      subgoal for rex l1
+        apply simp
+        apply (cases l1)
+        subgoal by fastforce
+        subgoal for op l1
+          apply simp
+          apply (cases l1)
+          subgoal by fastforce
+          subgoal for reg l1
+            apply simp
+            apply (cases r1; cases rd,auto simp add: bitfield_insert_u8_def Let_def ireg_of_u8_def)
+            done
+          done
+        done
+      done
+    done
+  done
+
+lemma x64assemble_disassemble_consistency_pnegl: "\<And>x20. (\<And>l_bin.
+               x64_assemble l_asm = Some l_bin \<Longrightarrow>
+               x64_disassemble l_bin = Some l_asm) \<Longrightarrow>
+           (case x64_assemble l_asm of None \<Rightarrow> None
+            | Some l \<Rightarrow>
+                Some
+                 ([or 64
+                    (construct_rex_to_u8 False False False
+                      (and (u8_of_ireg x20) 8 \<noteq> 0)),
+                   247, construct_modsib_to_u8 3 3 (u8_of_ireg x20)] @
+                  l)) =
+           Some l_bin \<Longrightarrow>
+           a = Pnegl x20 \<Longrightarrow> x64_disassemble l_bin = Some (Pnegl x20 # l_asm)"
+  subgoal for rd
+    apply (cases "x64_assemble l_asm")
+    subgoal by simp
+    subgoal for l1
+      apply simp
+      apply (unfold construct_rex_to_u8_def construct_modsib_to_u8_def)
+      apply simp
+      apply (cases l_bin)
+      subgoal by fastforce
+      subgoal for rex l1
+        apply (cases l1)
+        subgoal by fastforce
+        subgoal for op l1
+          apply simp
+          apply (cases l1)
+          subgoal by fastforce
+          subgoal for reg l1
+            apply simp
+            apply (cases rd, auto simp add: bitfield_insert_u8_def Let_def ireg_of_u8_def)
+            done
+          done
+        done
+      done
+    done
+  done
+
+lemma x64assemble_disassemble_consistency_pnegq: "\<And>x21a.
+       (\<And>l_bin. x64_assemble l_asm = Some l_bin \<Longrightarrow> x64_disassemble l_bin = Some l_asm) \<Longrightarrow>
+       (case x64_assemble l_asm of None \<Rightarrow> None
+        | Some l \<Rightarrow>
+            Some
+             ([or 64 (construct_rex_to_u8 True False False (and (u8_of_ireg x21a) 8 \<noteq> 0)), 247,
+               construct_modsib_to_u8 3 3 (u8_of_ireg x21a)] @
+              l)) =
+       Some l_bin \<Longrightarrow>
+       a = Pnegq x21a \<Longrightarrow> x64_disassemble l_bin = Some (Pnegq x21a # l_asm)"
+  subgoal for rd
+    apply (cases "x64_assemble l_asm")
+    subgoal by simp
+    subgoal for l1
+      apply simp
+      apply (unfold construct_rex_to_u8_def construct_modsib_to_u8_def)
+      apply simp
+      apply (cases l_bin)
+      subgoal by fastforce
+      subgoal for rex l1
+        apply (cases l1)
+        subgoal by fastforce
+        subgoal for op l1
+          apply simp
+          apply (cases l1)
+          subgoal by fastforce
+          subgoal for reg l1
+            apply simp
+            apply (cases rd, auto simp add: bitfield_insert_u8_def Let_def ireg_of_u8_def)
+            done
+          done
+        done
+      done
+    done
+  done
+
+lemma x64assemble_disassemble_consistency_paddq_rr :"\<And>x221 x222.
+       (\<And>l_bin. x64_assemble l_asm = Some l_bin \<Longrightarrow> x64_disassemble l_bin = Some l_asm) \<Longrightarrow>
+       (case x64_assemble l_asm of None \<Rightarrow> None
+        | Some l \<Rightarrow>
+            Some
+             ([or 64 (construct_rex_to_u8 True (and (u8_of_ireg x222) 8 \<noteq> 0) False (and (u8_of_ireg x221) 8 \<noteq> 0)),
+               1, construct_modsib_to_u8 3 (u8_of_ireg x222) (u8_of_ireg x221)] @
+              l)) =
+       Some l_bin \<Longrightarrow>
+       a = Paddq_rr x221 x222 \<Longrightarrow> x64_disassemble l_bin = Some (Paddq_rr x221 x222 # l_asm)"
+  subgoal for rd r1
+    apply (cases "x64_assemble l_asm")
+    subgoal by simp
+    subgoal for l1
+      apply simp
+      apply (unfold construct_rex_to_u8_def construct_modsib_to_u8_def)
+      apply simp
+      apply (cases l_bin)
+      subgoal by fastforce
+      subgoal for rex l1
+        apply (cases l1)
+        subgoal by fastforce
+        subgoal for op l1
+          apply simp
+          apply (cases l1)
+          subgoal by fastforce
+          subgoal for reg l1
+            apply simp
+            apply (cases r1; cases rd, auto simp add: bitfield_insert_u8_def Let_def ireg_of_u8_def)
+            done
+          done
+        done
+      done
+    done
+  done
+
+lemma x64assemble_disassemble_consistency_paddl_rr :"\<And>x231 x232.
+       (\<And>l_bin. x64_assemble l_asm = Some l_bin \<Longrightarrow> x64_disassemble l_bin = Some l_asm) \<Longrightarrow>
+       (case x64_assemble l_asm of None \<Rightarrow> None
+        | Some l \<Rightarrow>
+            Some
+             ([or 64
+                (construct_rex_to_u8 False (and (u8_of_ireg x232) 8 \<noteq> 0) False
+                  (and (u8_of_ireg x231) 8 \<noteq> 0)),
+               1, construct_modsib_to_u8 3 (u8_of_ireg x232) (u8_of_ireg x231)] @
+              l)) =
+       Some l_bin \<Longrightarrow>
+       a = Paddl_rr x231 x232 \<Longrightarrow> x64_disassemble l_bin = Some (Paddl_rr x231 x232 # l_asm)"
+  subgoal for rd r1
+    apply (cases "x64_assemble l_asm")
+    subgoal by simp
+    subgoal for l1
+      apply simp
+      apply (unfold construct_rex_to_u8_def construct_modsib_to_u8_def)
+      apply simp
+      apply (cases l_bin)
+      subgoal by fastforce
+      subgoal for rex l1
+        apply (cases l1)
+        subgoal by fastforce
+        subgoal for op l1
+          apply simp
+          apply (cases l1)
+          subgoal by fastforce
+          subgoal for reg l1
+            apply simp
+            apply (cases r1; cases rd, auto simp add: bitfield_insert_u8_def Let_def ireg_of_u8_def)
+            done
+          done
+        done
+      done
+    done
+  done
+
+
+lemma x64assemble_disassemble_consistency_psubl_rr: " \<And>x241 x242.
+       (\<And>l_bin. x64_assemble l_asm = Some l_bin \<Longrightarrow> x64_disassemble l_bin = Some l_asm) \<Longrightarrow>
+       (case x64_assemble l_asm of None \<Rightarrow> None
+        | Some l \<Rightarrow>
+            Some
+             ([or 64
+                (construct_rex_to_u8 False (and (u8_of_ireg x242) 8 \<noteq> 0) False
+                  (and (u8_of_ireg x241) 8 \<noteq> 0)),
+               41, construct_modsib_to_u8 3 (u8_of_ireg x242) (u8_of_ireg x241)] @
+              l)) =
+       Some l_bin \<Longrightarrow>
+       a = Psubl_rr x241 x242 \<Longrightarrow> x64_disassemble l_bin = Some (Psubl_rr x241 x242 # l_asm)"
+  subgoal for rd r1
+    apply (cases "x64_assemble l_asm")
+    subgoal by simp
+    subgoal for l1
+      apply simp
+      apply (unfold construct_rex_to_u8_def construct_modsib_to_u8_def)
+      apply simp
+      apply (cases l_bin)
+      subgoal by fastforce
+      subgoal for rex l1
+        apply (cases l1)
+        subgoal by fastforce
+        subgoal for op l1
+          apply simp
+          apply (cases l1)
+          subgoal by fastforce
+          subgoal for reg l1
+            apply simp
+            apply (cases r1; cases rd, auto simp add: bitfield_insert_u8_def Let_def ireg_of_u8_def)
+            done
+          done
+        done
+      done
+    done
+  done
+
+lemma x64assemble_disassemble_consistency_psubq_rr: "\<And>x251 x252.
+       (\<And>l_bin. x64_assemble l_asm = Some l_bin \<Longrightarrow> x64_disassemble l_bin = Some l_asm) \<Longrightarrow>
+       (case x64_assemble l_asm of None \<Rightarrow> None
+        | Some l \<Rightarrow>
+            Some
+             ([or 64 (construct_rex_to_u8 True (and (u8_of_ireg x252) 8 \<noteq> 0) False (and (u8_of_ireg x251) 8 \<noteq> 0)),
+               41, construct_modsib_to_u8 3 (u8_of_ireg x252) (u8_of_ireg x251)] @
+              l)) =
+       Some l_bin \<Longrightarrow>
+       a = Psubq_rr x251 x252 \<Longrightarrow> x64_disassemble l_bin = Some (Psubq_rr x251 x252 # l_asm)"
+  subgoal for rd r1
+    apply (cases "x64_assemble l_asm")
+    subgoal by simp
+    subgoal for l1
+      apply simp
+      apply (unfold construct_rex_to_u8_def construct_modsib_to_u8_def)
+      apply simp
+      apply (cases l_bin)
+      subgoal by fastforce
+      subgoal for rex l1
+        apply (cases l1)
+        subgoal by fastforce
+        subgoal for op l1
+          apply simp
+          apply (cases l1)
+          subgoal by fastforce
+          subgoal for reg l1
+            apply simp
+            apply (cases r1; cases rd, auto simp add: bitfield_insert_u8_def Let_def ireg_of_u8_def)
+            done
+          done
+        done
+      done
+    done
+  done
+
+lemma x64assemble_disassemble_consistency_pmull_r: "\<And>x26. 
+          (\<And>l_bin. x64_assemble l_asm = Some l_bin \<Longrightarrow> x64_disassemble l_bin = Some l_asm) \<Longrightarrow>
+           (case x64_assemble l_asm of None \<Rightarrow> None
+            | Some l \<Rightarrow>
+                Some
+                 ([or 64 (construct_rex_to_u8 False False False (and (u8_of_ireg x26) 8 \<noteq> 0)), 247,
+                   construct_modsib_to_u8 3 4 (u8_of_ireg x26)] @
+                  l)) =
+           Some l_bin \<Longrightarrow>
+           a = Pmull_r x26 \<Longrightarrow> x64_disassemble l_bin = Some (Pmull_r x26 # l_asm)"
+  subgoal for r1 
+    apply (cases "x64_assemble l_asm")
+    subgoal by simp
+    subgoal for l1
+      apply simp
+      apply (unfold construct_rex_to_u8_def construct_modsib_to_u8_def)
+      apply simp
+      apply (cases l_bin)
+      subgoal by fastforce
+      subgoal for rex l1
+        apply (cases l1)
+        subgoal by fastforce
+        subgoal for op l1
+          apply simp
+          apply (cases l1)
+          subgoal by fastforce
+          subgoal for reg l1
+            apply simp
+            apply (cases r1, auto simp add: bitfield_insert_u8_def Let_def ireg_of_u8_def)
+            done
+          done
+        done
+      done
+    done
+  done
+
+lemma x64assemble_disassemble_consistency_pmulq_r: "\<And>x27. 
+          (\<And>l_bin. x64_assemble l_asm = Some l_bin \<Longrightarrow> x64_disassemble l_bin = Some l_asm) \<Longrightarrow>
+           (case x64_assemble l_asm of None \<Rightarrow> None
+            | Some l \<Rightarrow>
+                Some
+                 ([or 64 (construct_rex_to_u8 True False False (and (u8_of_ireg x27) 8 \<noteq> 0)), 247,
+                   construct_modsib_to_u8 3 4 (u8_of_ireg x27)] @
+                  l)) =
+           Some l_bin \<Longrightarrow>
+           a = Pmulq_r x27 \<Longrightarrow> x64_disassemble l_bin = Some (Pmulq_r x27 # l_asm)"
+  subgoal for r1
+    apply (cases "x64_assemble l_asm")
+    subgoal by simp
+    subgoal for l1
+      apply simp
+      apply (unfold construct_rex_to_u8_def construct_modsib_to_u8_def)
+      apply simp
+      apply (cases l_bin)
+      subgoal by fastforce
+      subgoal for rex l1
+        apply (cases l1)
+        subgoal by fastforce
+        subgoal for op l1
+          apply simp
+          apply (cases l1)
+          subgoal by fastforce
+          subgoal for reg l1
+            apply simp
+            apply (cases r1, auto simp add: bitfield_insert_u8_def Let_def ireg_of_u8_def)
+            done
+          done
+        done
+      done
+    done
+  done
+
+lemma x64assemble_disassemble_consistency_pimull_r: "\<And>x28. 
+          (\<And>l_bin. x64_assemble l_asm = Some l_bin \<Longrightarrow> x64_disassemble l_bin = Some l_asm) \<Longrightarrow>
+           (case x64_assemble l_asm of None \<Rightarrow> None
+            | Some l \<Rightarrow>
+                Some
+                 ([or 64 (construct_rex_to_u8 False False False (and (u8_of_ireg x28) 8 \<noteq> 0)), 247,
+                   construct_modsib_to_u8 3 5 (u8_of_ireg x28)] @
+                  l)) =
+           Some l_bin \<Longrightarrow>
+           a = Pimull_r x28 \<Longrightarrow> x64_disassemble l_bin = Some (Pimull_r x28 # l_asm)"
+  subgoal for r1
+    apply (cases "x64_assemble l_asm")
+    subgoal by simp
+    subgoal for l1
+      apply simp
+      apply (unfold construct_rex_to_u8_def construct_modsib_to_u8_def)
+      apply simp
+      apply (cases l_bin)
+      subgoal by fastforce
+      subgoal for rex l1
+        apply (cases l1)
+        subgoal by fastforce
+        subgoal for op l1
+          apply simp
+          apply (cases l1)
+          subgoal by fastforce
+          subgoal for reg l1
+            apply simp
+            apply (cases r1, auto simp add: bitfield_insert_u8_def Let_def ireg_of_u8_def)
+            done
+          done
+        done
+      done
+    done
+  done
+
+lemma x64assemble_disassemble_consistency_pimulq_r: "\<And>x29.
+           (\<And>l_bin. x64_assemble l_asm = Some l_bin \<Longrightarrow> x64_disassemble l_bin = Some l_asm) \<Longrightarrow>
+           (case x64_assemble l_asm of None \<Rightarrow> None
+            | Some l \<Rightarrow>
+                Some
+                 ([or 64 (construct_rex_to_u8 True False False (and (u8_of_ireg x29) 8 \<noteq> 0)), 247,
+                   construct_modsib_to_u8 3 5 (u8_of_ireg x29)] @
+                  l)) =
+           Some l_bin \<Longrightarrow>
+           a = Pimulq_r x29 \<Longrightarrow> x64_disassemble l_bin = Some (Pimulq_r x29 # l_asm)"
+  subgoal for r1 
+    apply (cases "x64_assemble l_asm")
+    subgoal by simp
+    subgoal for l1
+      apply simp
+      apply (unfold construct_rex_to_u8_def construct_modsib_to_u8_def)
+      apply simp
+      apply (cases l_bin)
+      subgoal by fastforce
+      subgoal for rex l1
+        apply (cases l1)
+        subgoal by fastforce
+        subgoal for op l1
+          apply simp
+          apply (cases l1)
+          subgoal by fastforce
+          subgoal for reg l1
+            apply simp
+            apply (cases r1, auto simp add: bitfield_insert_u8_def Let_def ireg_of_u8_def)
+            done
+          done
+        done
+      done
+    done
+  done
+
+lemma x64assemble_disassemble_consistency_pdivl_r: "\<And>x30.
+     (\<And>l_bin. x64_assemble l_asm = Some l_bin \<Longrightarrow> x64_disassemble l_bin = Some l_asm) \<Longrightarrow>
+      (case x64_assemble l_asm of None \<Rightarrow> None
+       | Some l \<Rightarrow>
+           Some
+            ([or 64 (construct_rex_to_u8 False False False (and (u8_of_ireg x30) 8 \<noteq> 0)), 247,
+              construct_modsib_to_u8 3 6 (u8_of_ireg x30)] @
+             l)) =
+      Some l_bin \<Longrightarrow>
+      a = Pdivl_r x30 \<Longrightarrow> x64_disassemble l_bin = Some (Pdivl_r x30 # l_asm)"
+  subgoal for r1 
+    apply (cases "x64_assemble l_asm")
+    subgoal by simp
+    subgoal for l1
+      apply simp
+      apply (unfold construct_rex_to_u8_def construct_modsib_to_u8_def)
+      apply simp
+      apply (cases l_bin)
+      subgoal by fastforce
+      subgoal for rex l1
+        apply (cases l1)
+        subgoal by fastforce
+        subgoal for op l1
+          apply simp
+          apply (cases l1)
+          subgoal by fastforce
+          subgoal for reg l1
+            apply simp
+            apply (cases r1, auto simp add: bitfield_insert_u8_def Let_def ireg_of_u8_def)
+            done
+          done
+        done
+      done
+    done
+  done
+
+lemma x64assemble_disassemble_consistency_pdivq_r: "\<And>x31a.
+      (\<And>l_bin. x64_assemble l_asm = Some l_bin \<Longrightarrow> x64_disassemble l_bin = Some l_asm) \<Longrightarrow>
+      (case x64_assemble l_asm of None \<Rightarrow> None
+       | Some l \<Rightarrow>
+           Some
+            ([or 64 (construct_rex_to_u8 True False False (and (u8_of_ireg x31a) 8 \<noteq> 0)), 247,
+              construct_modsib_to_u8 3 6 (u8_of_ireg x31a)] @
+             l)) =
+      Some l_bin \<Longrightarrow>
+      a = Pdivq_r x31a \<Longrightarrow> x64_disassemble l_bin = Some (Pdivq_r x31a # l_asm)"
+  subgoal for r1
+    apply (cases "x64_assemble l_asm")
+    subgoal by simp
+    subgoal for l1
+      apply simp
+      apply (unfold construct_rex_to_u8_def construct_modsib_to_u8_def)
+      apply simp
+      apply (cases l_bin)
+      subgoal by fastforce
+      subgoal for rex l1
+        apply (cases l1)
+        subgoal by fastforce
+        subgoal for op l1
+          apply simp
+          apply (cases l1)
+          subgoal by fastforce
+          subgoal for reg l1
+            apply simp
+            apply (cases r1, auto simp add: bitfield_insert_u8_def Let_def ireg_of_u8_def)
+            done
+          done
+        done
+      done
+    done
+  done
+
+lemma x64assemble_disassemble_consistency_pidivl_r: "\<And>x32a.
+      (\<And>l_bin. x64_assemble l_asm = Some l_bin \<Longrightarrow> x64_disassemble l_bin = Some l_asm) \<Longrightarrow>
+      (case x64_assemble l_asm of None \<Rightarrow> None
+       | Some l \<Rightarrow>
+           Some
+            ([or 64 (construct_rex_to_u8 False False False (and (u8_of_ireg x32a) 8 \<noteq> 0)), 247,
+              construct_modsib_to_u8 3 7 (u8_of_ireg x32a)] @
+             l)) =
+      Some l_bin \<Longrightarrow>
+      a = Pidivl_r x32a \<Longrightarrow> x64_disassemble l_bin = Some (Pidivl_r x32a # l_asm)"
+  subgoal for r1
+    apply (cases "x64_assemble l_asm")
+    subgoal by simp
+    subgoal for l1
+      apply simp
+      apply (unfold construct_rex_to_u8_def construct_modsib_to_u8_def)
+      apply simp
+      apply (cases l_bin)
+      subgoal by fastforce
+      subgoal for rex l1
+        apply (cases l1)
+        subgoal by fastforce
+        subgoal for op l1
+          apply simp
+          apply (cases l1)
+          subgoal by fastforce
+          subgoal for reg l1
+            apply simp
+            apply (cases r1, auto simp add: bitfield_insert_u8_def Let_def ireg_of_u8_def)
+            done
+          done
+        done
+      done
+    done
+  done
+
+lemma x64assemble_disassemble_consistency_pidivq_r: "\<And>x33. 
+      (\<And>l_bin. x64_assemble l_asm = Some l_bin \<Longrightarrow> x64_disassemble l_bin = Some l_asm) \<Longrightarrow>
+      (case x64_assemble l_asm of None \<Rightarrow> None
+       | Some l \<Rightarrow>
+           Some
+            ([or 64 (construct_rex_to_u8 True False False (and (u8_of_ireg x33) 8 \<noteq> 0)), 247,
+              construct_modsib_to_u8 3 7 (u8_of_ireg x33)] @
+             l)) =
+      Some l_bin \<Longrightarrow>
+      a = Pidivq_r x33 \<Longrightarrow> x64_disassemble l_bin = Some (Pidivq_r x33 # l_asm)"
+  subgoal for r1 
+    apply (cases "x64_assemble l_asm")
+    subgoal by simp
+    subgoal for l1
+      apply simp
+      apply (unfold construct_rex_to_u8_def construct_modsib_to_u8_def)
+      apply simp
+      apply (cases l_bin)
+      subgoal by fastforce
+      subgoal for rex l1
+        apply (cases l1)
+        subgoal by fastforce
+        subgoal for op l1
+          apply simp
+          apply (cases l1)
+          subgoal by fastforce
+          subgoal for reg l1
+            apply simp
+            apply (cases r1, auto simp add: bitfield_insert_u8_def Let_def ireg_of_u8_def)
+            done
+          done
+        done
+      done
+    done
+  done
+
+lemma x64assemble_disassemble_consistency_pandl_rr :"\<And>x341 x342.
+       (\<And>l_bin. x64_assemble l_asm = Some l_bin \<Longrightarrow> x64_disassemble l_bin = Some l_asm) \<Longrightarrow>
+       (case x64_assemble l_asm of None \<Rightarrow> None
+        | Some l \<Rightarrow>
+            Some
+             ([or 64
+                (construct_rex_to_u8 False (and (u8_of_ireg x342) 8 \<noteq> 0) False
+                  (and (u8_of_ireg x341) 8 \<noteq> 0)),
+               33, construct_modsib_to_u8 3 (u8_of_ireg x342) (u8_of_ireg x341)] @
+              l)) =
+       Some l_bin \<Longrightarrow>
+       a = Pandl_rr x341 x342 \<Longrightarrow> x64_disassemble l_bin = Some (Pandl_rr x341 x342 # l_asm)"
+  subgoal for rd r1
+    apply (cases "x64_assemble l_asm")
+    subgoal by simp
+    subgoal for l1
+      apply simp
+      apply (unfold construct_rex_to_u8_def construct_modsib_to_u8_def)
+      apply simp
+      apply (cases l_bin)
+      subgoal by fastforce
+      subgoal for rex l1
+        apply (cases l1)
+        subgoal by fastforce
+        subgoal for op l1
+          apply simp
+          apply (cases l1)
+          subgoal by fastforce
+          subgoal for reg l1
+            apply simp
+            apply (cases r1; cases rd, auto simp add: bitfield_insert_u8_def Let_def ireg_of_u8_def)
+            done
+          done
+        done
+      done
+    done
+  done
+
+lemma x64assemble_disassemble_consistency_pandq_rr :"\<And>x351 x352.
+      (\<And>l_bin. x64_assemble l_asm = Some l_bin \<Longrightarrow> x64_disassemble l_bin = Some l_asm) \<Longrightarrow>
+      (case x64_assemble l_asm of None \<Rightarrow> None
+       | Some l \<Rightarrow>
+           Some
+            ([or 64
+               (construct_rex_to_u8 True (and (u8_of_ireg x352) 8 \<noteq> 0) False
+                 (and (u8_of_ireg x351) 8 \<noteq> 0)),
+              33, construct_modsib_to_u8 3 (u8_of_ireg x352) (u8_of_ireg x351)] @
+             l)) =
+      Some l_bin \<Longrightarrow>
+      a = Pandq_rr x351 x352 \<Longrightarrow> x64_disassemble l_bin = Some (Pandq_rr x351 x352 # l_asm)"
+  subgoal for rd r1
+    apply (cases "x64_assemble l_asm")
+    subgoal by simp
+    subgoal for l1
+      apply simp
+      apply (unfold construct_rex_to_u8_def construct_modsib_to_u8_def)
+      apply simp
+      apply (cases l_bin)
+      subgoal by fastforce
+      subgoal for rex l1
+        apply (cases l1)
+        subgoal by fastforce
+        subgoal for op l1
+          apply simp
+          apply (cases l1)
+          subgoal by fastforce
+          subgoal for reg l1
+            apply simp
+            apply (cases r1; cases rd, auto simp add: bitfield_insert_u8_def Let_def ireg_of_u8_def)
+            done
+          done
+        done
+      done
+    done
+  done
+
+lemma x64assemble_disassemble_consistency_porl_rr :"\<And>x361 x362.
+      (\<And>l_bin. x64_assemble l_asm = Some l_bin \<Longrightarrow> x64_disassemble l_bin = Some l_asm) \<Longrightarrow>
+      (case x64_assemble l_asm of None \<Rightarrow> None
+       | Some l \<Rightarrow>
+           Some
+            ([or 64
+               (construct_rex_to_u8 False (and (u8_of_ireg x362) 8 \<noteq> 0) False
+                 (and (u8_of_ireg x361) 8 \<noteq> 0)),
+              9, construct_modsib_to_u8 3 (u8_of_ireg x362) (u8_of_ireg x361)] @
+             l)) =
+      Some l_bin \<Longrightarrow>
+      a = Porl_rr x361 x362 \<Longrightarrow> x64_disassemble l_bin = Some (Porl_rr x361 x362 # l_asm)"
+  subgoal for rd r1
+    apply (cases "x64_assemble l_asm")
+    subgoal by simp
+    subgoal for l1
+      apply simp
+      apply (unfold construct_rex_to_u8_def construct_modsib_to_u8_def)
+      apply simp
+      apply (cases l_bin)
+      subgoal by fastforce
+      subgoal for rex l1
+        apply (cases l1)
+        subgoal by fastforce
+        subgoal for op l1
+          apply simp
+          apply (cases l1)
+          subgoal by fastforce
+          subgoal for reg l1
+            apply simp
+            apply (cases r1; cases rd, auto simp add: bitfield_insert_u8_def Let_def ireg_of_u8_def)
+            done
+          done
+        done
+      done
+    done
+  done
+
+lemma x64assemble_disassemble_consistency_porq_rr :"\<And>x371 x372.
+      (\<And>l_bin. x64_assemble l_asm = Some l_bin \<Longrightarrow> x64_disassemble l_bin = Some l_asm) \<Longrightarrow>
+      (case x64_assemble l_asm of None \<Rightarrow> None
+       | Some l \<Rightarrow>
+           Some
+            ([or 64
+               (construct_rex_to_u8 True (and (u8_of_ireg x372) 8 \<noteq> 0) False
+                 (and (u8_of_ireg x371) 8 \<noteq> 0)),
+              9, construct_modsib_to_u8 3 (u8_of_ireg x372) (u8_of_ireg x371)] @
+             l)) =
+      Some l_bin \<Longrightarrow>
+      a = Porq_rr x371 x372 \<Longrightarrow> x64_disassemble l_bin = Some (Porq_rr x371 x372 # l_asm)"
+  subgoal for rd r1
+    apply (cases "x64_assemble l_asm")
+    subgoal by simp
+    subgoal for l1
+      apply simp
+      apply (unfold construct_rex_to_u8_def construct_modsib_to_u8_def)
+      apply simp
+      apply (cases l_bin)
+      subgoal by fastforce
+      subgoal for rex l1
+        apply (cases l1)
+        subgoal by fastforce
+        subgoal for op l1
+          apply simp
+          apply (cases l1)
+          subgoal by fastforce
+          subgoal for reg l1
+            apply simp
+            apply (cases r1; cases rd, auto simp add: bitfield_insert_u8_def Let_def ireg_of_u8_def)
+            done
+          done
+        done
+      done
+    done
+  done
+
+lemma x64assemble_disassemble_consistency_pxorl_rr :"\<And>x381 x382.
+      (\<And>l_bin. x64_assemble l_asm = Some l_bin \<Longrightarrow> x64_disassemble l_bin = Some l_asm) \<Longrightarrow>
+      (case x64_assemble l_asm of None \<Rightarrow> None
+       | Some l \<Rightarrow>
+           Some
+            ([or 64
+               (construct_rex_to_u8 False (and (u8_of_ireg x382) 8 \<noteq> 0) False
+                 (and (u8_of_ireg x381) 8 \<noteq> 0)),
+              49, construct_modsib_to_u8 3 (u8_of_ireg x382) (u8_of_ireg x381)] @
+             l)) =
+      Some l_bin \<Longrightarrow>
+      a = Pxorl_rr x381 x382 \<Longrightarrow> x64_disassemble l_bin = Some (Pxorl_rr x381 x382 # l_asm)"
+  subgoal for rd r1
+    apply (cases "x64_assemble l_asm")
+    subgoal by simp
+    subgoal for l1
+      apply simp
+      apply (unfold construct_rex_to_u8_def construct_modsib_to_u8_def)
+      apply simp
+      apply (cases l_bin)
+      subgoal by fastforce
+      subgoal for rex l1
+        apply (cases l1)
+        subgoal by fastforce
+        subgoal for op l1
+          apply simp
+          apply (cases l1)
+          subgoal by fastforce
+          subgoal for reg l1
+            apply simp
+            apply (cases r1; cases rd, auto simp add: bitfield_insert_u8_def Let_def ireg_of_u8_def)
+            done
+          done
+        done
+      done
+    done
+  done
+
+lemma x64assemble_disassemble_consistency_pxorq_rr :"\<And>x391 x392.
+    (\<And>l_bin. x64_assemble l_asm = Some l_bin \<Longrightarrow> x64_disassemble l_bin = Some l_asm) \<Longrightarrow>
+    (case x64_assemble l_asm of None \<Rightarrow> None
+     | Some l \<Rightarrow>
+         Some
+          ([or 64
+             (construct_rex_to_u8 True (and (u8_of_ireg x392) 8 \<noteq> 0) False
+               (and (u8_of_ireg x391) 8 \<noteq> 0)),
+            49, construct_modsib_to_u8 3 (u8_of_ireg x392) (u8_of_ireg x391)] @
+           l)) =
+    Some l_bin \<Longrightarrow>
+    a = Pxorq_rr x391 x392 \<Longrightarrow> x64_disassemble l_bin = Some (Pxorq_rr x391 x392 # l_asm)"
+  subgoal for rd r1
+    apply (cases "x64_assemble l_asm")
+    subgoal by simp
+    subgoal for l1
+      apply simp
+      apply (unfold construct_rex_to_u8_def construct_modsib_to_u8_def)
+      apply simp
+      apply (cases l_bin)
+      subgoal by fastforce
+      subgoal for rex l1
+        apply (cases l1)
+        subgoal by fastforce
+        subgoal for op l1
+          apply simp
+          apply (cases l1)
+          subgoal by fastforce
+          subgoal for reg l1
+            apply simp
+            apply (cases r1; cases rd, auto simp add: bitfield_insert_u8_def Let_def ireg_of_u8_def)
+            done
+          done
+        done
+      done
+    done
+  done
+
+lemma x64assemble_disassemble_consistency_pshll_ri :"\<And>x401 x402.
+      (\<And>l_bin. x64_assemble l_asm = Some l_bin \<Longrightarrow> x64_disassemble l_bin = Some l_asm) \<Longrightarrow>
+      (case x64_assemble l_asm of None \<Rightarrow> None
+       | Some l \<Rightarrow>
+           Some
+            ([or 64 (construct_rex_to_u8 False False False (and (u8_of_ireg x401) 8 \<noteq> 0)), 193,
+              construct_modsib_to_u8 3 4 (u8_of_ireg x401), x402] @
+             l)) =
+      Some l_bin \<Longrightarrow>
+      a = Pshll_ri x401 x402 \<Longrightarrow> x64_disassemble l_bin = Some (Pshll_ri x401 x402 # l_asm)"
+  subgoal for rd n
+    apply (cases "x64_assemble l_asm")
+    subgoal by simp
+    subgoal for l1
+      apply simp
+      apply (unfold construct_rex_to_u8_def construct_modsib_to_u8_def)
+      apply simp
+      apply (cases l_bin)
+      subgoal by fastforce
+      subgoal for rex l1
+        apply (cases l1)
+        subgoal by fastforce
+        subgoal for op l1
+          apply simp
+          apply (cases l1)
+          subgoal by fastforce
+          subgoal for reg l1
+            apply simp
+            apply (cases n; cases rd, auto simp add: bitfield_insert_u8_def Let_def ireg_of_u8_def)
+            done                               
+          done
+        done
+      done
+    done
+  done
+
+lemma x64assemble_disassemble_consistency_pshlq_ri :"\<And>x411 x412.
+      (\<And>l_bin. x64_assemble l_asm = Some l_bin \<Longrightarrow> x64_disassemble l_bin = Some l_asm) \<Longrightarrow>
+      (case x64_assemble l_asm of None \<Rightarrow> None
+       | Some l \<Rightarrow>
+           Some
+            ([or 64 (construct_rex_to_u8 True False False (and (u8_of_ireg x411) 8 \<noteq> 0)), 193,
+              construct_modsib_to_u8 3 4 (u8_of_ireg x411), x412] @
+             l)) =
+      Some l_bin \<Longrightarrow>
+      a = Pshlq_ri x411 x412 \<Longrightarrow> x64_disassemble l_bin = Some (Pshlq_ri x411 x412 # l_asm)"
+  subgoal for rd n
+    apply (cases "x64_assemble l_asm")
+    subgoal by simp
+    subgoal for l1
+      apply simp
+      apply (unfold construct_rex_to_u8_def construct_modsib_to_u8_def)
+      apply simp
+      apply (cases l_bin)
+      subgoal by fastforce
+      subgoal for rex l1
+        apply (cases l1)
+        subgoal by fastforce
+        subgoal for op l1
+          apply simp
+          apply (cases l1)
+          subgoal by fastforce
+          subgoal for reg l1
+            apply simp
+            apply (cases n; cases rd, auto simp add: bitfield_insert_u8_def Let_def ireg_of_u8_def)
+            done                               
+          done
+        done
+      done
+    done
+  done
+
+lemma x64assemble_disassemble_consistency_pshll_r :"\<And>x42a.
+      (\<And>l_bin. x64_assemble l_asm = Some l_bin \<Longrightarrow> x64_disassemble l_bin = Some l_asm) \<Longrightarrow>
+      (case x64_assemble l_asm of None \<Rightarrow> None
+       | Some l \<Rightarrow>
+           Some
+            ([or 64 (construct_rex_to_u8 False False False (and (u8_of_ireg x42a) 8 \<noteq> 0)), 211,
+              construct_modsib_to_u8 3 4 (u8_of_ireg x42a)] @
+             l)) =
+      Some l_bin \<Longrightarrow>
+      a = Pshll_r x42a \<Longrightarrow> x64_disassemble l_bin = Some (Pshll_r x42a # l_asm)"
+  subgoal for rd 
+    apply (cases "x64_assemble l_asm")
+    subgoal by simp
+    subgoal for l1
+      apply simp
+      apply (unfold construct_rex_to_u8_def construct_modsib_to_u8_def)
+      apply simp
+      apply (cases l_bin)
+      subgoal by fastforce
+      subgoal for rex l1
+        apply (cases l1)
+        subgoal by fastforce
+        subgoal for op l1
+          apply simp
+          apply (cases l1)
+          subgoal by fastforce
+          subgoal for reg l1
+            apply simp
+            apply ( cases rd, auto simp add: bitfield_insert_u8_def Let_def ireg_of_u8_def)
+            done                               
+          done
+        done
+      done
+    done
+  done
+
+lemma x64assemble_disassemble_consistency_pshlq_r :"\<And>x43. 
+      (\<And>l_bin. x64_assemble l_asm = Some l_bin \<Longrightarrow> x64_disassemble l_bin = Some l_asm) \<Longrightarrow>
+      (case x64_assemble l_asm of None \<Rightarrow> None
+       | Some l \<Rightarrow>
+           Some
+            ([or 64 (construct_rex_to_u8 True False False (and (u8_of_ireg x43) 8 \<noteq> 0)), 211,
+              construct_modsib_to_u8 3 4 (u8_of_ireg x43)] @
+             l)) =
+      Some l_bin \<Longrightarrow>
+      a = Pshlq_r x43 \<Longrightarrow> x64_disassemble l_bin = Some (Pshlq_r x43 # l_asm)"
+  subgoal for rd 
+    apply (cases "x64_assemble l_asm")
+    subgoal by simp
+    subgoal for l1
+      apply simp
+      apply (unfold construct_rex_to_u8_def construct_modsib_to_u8_def)
+      apply simp
+      apply (cases l_bin)
+      subgoal by fastforce
+      subgoal for rex l1
+        apply (cases l1)
+        subgoal by fastforce
+        subgoal for op l1
+          apply simp
+          apply (cases l1)
+          subgoal by fastforce
+          subgoal for reg l1
+            apply simp
+            apply ( cases rd, auto simp add: bitfield_insert_u8_def Let_def ireg_of_u8_def)
+            done                               
+          done
+        done
+      done
+    done
+  done
+
+lemma x64assemble_disassemble_consistency_pshrl_ri :"\<And>x441 x442.
+     (\<And>l_bin. x64_assemble l_asm = Some l_bin \<Longrightarrow> x64_disassemble l_bin = Some l_asm) \<Longrightarrow>
+     (case x64_assemble l_asm of None \<Rightarrow> None
+      | Some l \<Rightarrow>
+          Some
+           ([or 64 (construct_rex_to_u8 False False False (and (u8_of_ireg x441) 8 \<noteq> 0)), 193,
+             construct_modsib_to_u8 3 5 (u8_of_ireg x441), x442] @
+            l)) =
+     Some l_bin \<Longrightarrow>
+     a = Pshrl_ri x441 x442 \<Longrightarrow> x64_disassemble l_bin = Some (Pshrl_ri x441 x442 # l_asm)"
+  subgoal for rd n
+    apply (cases "x64_assemble l_asm")
+    subgoal by simp
+    subgoal for l1
+      apply simp
+      apply (unfold construct_rex_to_u8_def construct_modsib_to_u8_def)
+      apply simp
+      apply (cases l_bin)
+      subgoal by fastforce
+      subgoal for rex l1
+        apply (cases l1)
+        subgoal by fastforce
+        subgoal for op l1
+          apply simp
+          apply (cases l1)
+          subgoal by fastforce
+          subgoal for reg l1
+            apply simp
+            apply (cases n; cases rd, auto simp add: bitfield_insert_u8_def Let_def ireg_of_u8_def)
+            done                               
+          done
+        done
+      done
+    done
+  done
+
+lemma x64assemble_disassemble_consistency_pshrq_ri :"\<And>x451 x452.
+     (\<And>l_bin. x64_assemble l_asm = Some l_bin \<Longrightarrow> x64_disassemble l_bin = Some l_asm) \<Longrightarrow>
+     (case x64_assemble l_asm of None \<Rightarrow> None
+      | Some l \<Rightarrow>
+          Some
+           ([or 64 (construct_rex_to_u8 True False False (and (u8_of_ireg x451) 8 \<noteq> 0)), 193,
+             construct_modsib_to_u8 3 5 (u8_of_ireg x451), x452] @
+            l)) =
+     Some l_bin \<Longrightarrow>
+     a = Pshrq_ri x451 x452 \<Longrightarrow> x64_disassemble l_bin = Some (Pshrq_ri x451 x452 # l_asm)"
+  subgoal for rd n
+    apply (cases "x64_assemble l_asm")
+    subgoal by simp
+    subgoal for l1
+      apply simp
+      apply (unfold construct_rex_to_u8_def construct_modsib_to_u8_def)
+      apply simp
+      apply (cases l_bin)
+      subgoal by fastforce
+      subgoal for rex l1
+        apply (cases l1)
+        subgoal by fastforce
+        subgoal for op l1
+          apply simp
+          apply (cases l1)
+          subgoal by fastforce
+          subgoal for reg l1
+            apply simp
+            apply (cases n; cases rd, auto simp add: bitfield_insert_u8_def Let_def ireg_of_u8_def)
+            done                               
+          done
+        done
+      done
+    done
+  done
+
+lemma x64assemble_disassemble_consistency_pshrl_r :"\<And>x46. 
+      (\<And>l_bin. x64_assemble l_asm = Some l_bin \<Longrightarrow> x64_disassemble l_bin = Some l_asm) \<Longrightarrow>
+      (case x64_assemble l_asm of None \<Rightarrow> None
+       | Some l \<Rightarrow>
+           Some
+            ([or 64 (construct_rex_to_u8 False False False (and (u8_of_ireg x46) 8 \<noteq> 0)), 211,
+              construct_modsib_to_u8 3 5 (u8_of_ireg x46)] @
+             l)) =
+      Some l_bin \<Longrightarrow>
+      a = Pshrl_r x46 \<Longrightarrow> x64_disassemble l_bin = Some (Pshrl_r x46 # l_asm)"
+  subgoal for rd 
+    apply (cases "x64_assemble l_asm")
+    subgoal by simp
+    subgoal for l1
+      apply simp
+      apply (unfold construct_rex_to_u8_def construct_modsib_to_u8_def)
+      apply simp
+      apply (cases l_bin)
+      subgoal by fastforce
+      subgoal for rex l1
+        apply (cases l1)
+        subgoal by fastforce
+        subgoal for op l1
+          apply simp
+          apply (cases l1)
+          subgoal by fastforce
+          subgoal for reg l1
+            apply simp
+            apply ( cases rd, auto simp add: bitfield_insert_u8_def Let_def ireg_of_u8_def)
+            done                               
+          done
+        done
+      done
+    done
+  done
+
+lemma x64assemble_disassemble_consistency_pshrq_r :"\<And>x47. 
+      (\<And>l_bin. x64_assemble l_asm = Some l_bin \<Longrightarrow> x64_disassemble l_bin = Some l_asm) \<Longrightarrow>
+      (case x64_assemble l_asm of None \<Rightarrow> None
+       | Some l \<Rightarrow>
+           Some
+            ([or 64 (construct_rex_to_u8 True False False (and (u8_of_ireg x47) 8 \<noteq> 0)), 211,
+              construct_modsib_to_u8 3 5 (u8_of_ireg x47)] @
+             l)) =
+      Some l_bin \<Longrightarrow>
+      a = Pshrq_r x47 \<Longrightarrow> x64_disassemble l_bin = Some (Pshrq_r x47 # l_asm)"
+  subgoal for rd 
+    apply (cases "x64_assemble l_asm")
+    subgoal by simp
+    subgoal for l1
+      apply simp
+      apply (unfold construct_rex_to_u8_def construct_modsib_to_u8_def)
+      apply simp
+      apply (cases l_bin)
+      subgoal by fastforce
+      subgoal for rex l1
+        apply (cases l1)
+        subgoal by fastforce
+        subgoal for op l1
+          apply simp
+          apply (cases l1)
+          subgoal by fastforce
+          subgoal for reg l1
+            apply simp
+            apply ( cases rd, auto simp add: bitfield_insert_u8_def Let_def ireg_of_u8_def)
+            done                               
+          done
+        done
+      done
+    done
+  done
+
+lemma x64assemble_disassemble_consistency_psarl_ri :"\<And>x481 x482.
+      (\<And>l_bin. x64_assemble l_asm = Some l_bin \<Longrightarrow> x64_disassemble l_bin = Some l_asm) \<Longrightarrow>
+      (case x64_assemble l_asm of None \<Rightarrow> None
+       | Some l \<Rightarrow>
+           Some
+            ([or 64 (construct_rex_to_u8 False False False (and (u8_of_ireg x481) 8 \<noteq> 0)), 193,
+              construct_modsib_to_u8 3 7 (u8_of_ireg x481), x482] @
+             l)) =
+      Some l_bin \<Longrightarrow>
+      a = Psarl_ri x481 x482 \<Longrightarrow> x64_disassemble l_bin = Some (Psarl_ri x481 x482 # l_asm)"
+  subgoal for rd n
+    apply (cases "x64_assemble l_asm")
+    subgoal by simp
+    subgoal for l1
+      apply simp
+      apply (unfold construct_rex_to_u8_def construct_modsib_to_u8_def)
+      apply simp
+      apply (cases l_bin)
+      subgoal by fastforce
+      subgoal for rex l1
+        apply (cases l1)
+        subgoal by fastforce
+        subgoal for op l1
+          apply simp
+          apply (cases l1)
+          subgoal by fastforce
+          subgoal for reg l1
+            apply simp
+            apply (cases n; cases rd, auto simp add: bitfield_insert_u8_def Let_def ireg_of_u8_def)
+            done                               
+          done
+        done
+      done
+    done
+  done
+
+lemma x64assemble_disassemble_consistency_psarq_ri :"\<And>x491 x492.
+      (\<And>l_bin. x64_assemble l_asm = Some l_bin \<Longrightarrow> x64_disassemble l_bin = Some l_asm) \<Longrightarrow>
+      (case x64_assemble l_asm of None \<Rightarrow> None
+       | Some l \<Rightarrow>
+           Some
+            ([or 64 (construct_rex_to_u8 True False False (and (u8_of_ireg x491) 8 \<noteq> 0)), 193,
+              construct_modsib_to_u8 3 7 (u8_of_ireg x491), x492] @
+             l)) =
+      Some l_bin \<Longrightarrow>
+      a = Psarq_ri x491 x492 \<Longrightarrow> x64_disassemble l_bin = Some (Psarq_ri x491 x492 # l_asm)"
+  subgoal for rd n
+    apply (cases "x64_assemble l_asm")
+    subgoal by simp
+    subgoal for l1
+      apply simp
+      apply (unfold construct_rex_to_u8_def construct_modsib_to_u8_def)
+      apply simp
+      apply (cases l_bin)
+      subgoal by fastforce
+      subgoal for rex l1
+        apply (cases l1)
+        subgoal by fastforce
+        subgoal for op l1
+          apply simp
+          apply (cases l1)
+          subgoal by fastforce
+          subgoal for reg l1
+            apply simp
+            apply (cases n; cases rd, auto simp add: bitfield_insert_u8_def Let_def ireg_of_u8_def)
+            done                               
+          done
+        done
+      done
+    done
+  done
+
+lemma x64assemble_disassemble_consistency_psarl_r :"\<And>x50. 
+    (\<And>l_bin. x64_assemble l_asm = Some l_bin \<Longrightarrow> x64_disassemble l_bin = Some l_asm) \<Longrightarrow>
+    (case x64_assemble l_asm of None \<Rightarrow> None
+     | Some l \<Rightarrow>
+         Some
+          ([or 64 (construct_rex_to_u8 False False False (and (u8_of_ireg x50) 8 \<noteq> 0)), 211,
+            construct_modsib_to_u8 3 7 (u8_of_ireg x50)] @
+           l)) =
+    Some l_bin \<Longrightarrow>
+    a = Psarl_r x50 \<Longrightarrow> x64_disassemble l_bin = Some (Psarl_r x50 # l_asm)"
+  subgoal for rd 
+    apply (cases "x64_assemble l_asm")
+    subgoal by simp
+    subgoal for l1
+      apply simp
+      apply (unfold construct_rex_to_u8_def construct_modsib_to_u8_def)
+      apply simp
+      apply (cases l_bin)
+      subgoal by fastforce
+      subgoal for rex l1
+        apply (cases l1)
+        subgoal by fastforce
+        subgoal for op l1
+          apply simp
+          apply (cases l1)
+          subgoal by fastforce
+          subgoal for reg l1
+            apply simp
+            apply ( cases rd, auto simp add: bitfield_insert_u8_def Let_def ireg_of_u8_def)
+            done                               
+          done
+        done
+      done
+    done
+  done
+
+lemma x64assemble_disassemble_consistency_psarq_r :"\<And>x51a.
+      (\<And>l_bin. x64_assemble l_asm = Some l_bin \<Longrightarrow> x64_disassemble l_bin = Some l_asm) \<Longrightarrow>
+      (case x64_assemble l_asm of None \<Rightarrow> None
+       | Some l \<Rightarrow>
+           Some
+            ([or 64 (construct_rex_to_u8 True False False (and (u8_of_ireg x51a) 8 \<noteq> 0)), 211,
+              construct_modsib_to_u8 3 7 (u8_of_ireg x51a)] @
+             l)) =
+      Some l_bin \<Longrightarrow>
+      a = Psarq_r x51a \<Longrightarrow> x64_disassemble l_bin = Some (Psarq_r x51a # l_asm)"
+  subgoal for rd 
+    apply (cases "x64_assemble l_asm")
+    subgoal by simp
+    subgoal for l1
+      apply simp
+      apply (unfold construct_rex_to_u8_def construct_modsib_to_u8_def)
+      apply simp
+      apply (cases l_bin)
+      subgoal by fastforce
+      subgoal for rex l1
+        apply (cases l1)
+        subgoal by fastforce
+        subgoal for op l1
+          apply simp
+          apply (cases l1)
+          subgoal by fastforce
+          subgoal for reg l1
+            apply simp
+            apply ( cases rd, auto simp add: bitfield_insert_u8_def Let_def ireg_of_u8_def)
+            done                               
+          done
+        done
+      done
+    done
+  done
+
+end
